cfrontend/ClightC.v
@@ -1,0 +1,185 @@
+Require Import CoqlibC.
+Require Import Errors.
+Require Import Maps.
+Require Import Integers.
+Require Import Floats.
+Require Import ValuesC.
+Require Import AST.
+Require Import Memory.
+Require Import Events.
+Require Import Globalenvs.
+Require Import Smallstep.
+Require Import CtypesC.
+Require Import Cop.
+(** newly added **)
+Require Import sflib.
+Require Import Clight.
+Require Import Skeleton Mod ModSem.
+Require Import CtypesC.
+Require Import CtypingC.
+
+Set Implicit Arguments.
+
+(* copied from Cshmgen *)
+Definition signature_of_function (fd: function) :=
+  {| sig_args := map typ_of_type (map snd (fn_params fd));
+     sig_res  := opttyp_of_type (fn_return fd);
+     sig_cc   := fn_callconv fd |}.
+
+Section MODSEM.
+
+  Variable skenv_link: SkEnv.t.
+  Variable p: program.
+  Let skenv: SkEnv.t := skenv_link.(SkEnv.project) p.(defs).
+  Let ge: genv := Build_genv (skenv.(CtypesC.revive) p) p.(prog_comp_env).
+
+  Inductive at_external: state -> Args.t -> Prop :=
+  | at_external_intro
+      fptr_arg sg_arg tyf vs_arg k0 m0
+      targs tres cconv
+      (EXTERNAL: ge.(Genv.find_funct) fptr_arg = None)
+      (SIG: exists skd, skenv_link.(Genv.find_funct) fptr_arg = Some skd
+                   /\ (SkEnv.get_sig skd = sg_arg
+                      -> tyf = Tfunction targs tres cconv
+                      -> signature_of_type targs tres cconv = sg_arg))
+    :
+      at_external (Callstate fptr_arg tyf vs_arg k0 m0)
+                  (Args.mk fptr_arg vs_arg m0)
+  .
+
+  Inductive initial_frame (args: Args.t)
+    : state -> Prop :=
+  | initial_frame_intro
+      tvs fd tyf
+      (FINDF: Genv.find_funct ge args.(Args.fptr) = Some (Internal fd))
+      (TYPE: type_of_fundef (Internal fd) = tyf) (* TODO: rename this into sig *)
+      (TYP: typecheck args.(Args.vs) (signature_of_function fd) tvs)
+    :
+      initial_frame args
+                    (Callstate args.(Args.fptr) tyf tvs Kstop args.(Args.m))
+  .
+
+  Inductive final_frame: state -> Retv.t -> Prop :=
+  | final_frame_intro
+      v_ret m_ret
+    :
+      final_frame (Returnstate v_ret Kstop m_ret) (Retv.mk v_ret m_ret)
+  .
+
+  Inductive after_external: state -> Retv.t -> state -> Prop :=
+  | after_external_intro
+      fptr_arg vs_arg m_arg
+      k retv tv
+      (* tyf *)
+      targs tres cconv
+      (TYP: typify_c retv.(Retv.v) tres tv)
+    :
+      after_external (Callstate fptr_arg (Tfunction targs tres cconv) vs_arg k m_arg)
+                     retv
+                     (Returnstate tv k retv.(Retv.m))
+  .
+
+  Program Definition modsem1: ModSem.t :=
+    {|
+      ModSem.step := step1;
+      ModSem.at_external := at_external;
+      ModSem.initial_frame := initial_frame;
+      ModSem.final_frame := final_frame;
+      ModSem.after_external := after_external;
+      ModSem.globalenv := ge;
+      ModSem.skenv := skenv;
+    |}
+  .
+  Next Obligation. ii; ss; des. inv_all_once; ss; clarify. Qed.
+  Next Obligation. ii; ss; des. inv_all_once; ss; clarify. Qed.
+  Next Obligation. ii; ss; des. inv_all_once; ss; clarify. f_equal. determ_tac typify_c_dtm. Qed.
+  Next Obligation. ii; ss; des. inv_all_once; ss; clarify. Qed.
+  Next Obligation. ii; ss; des. inv_all_once; ss; clarify. Qed.
+  Next Obligation. ii; ss; des. inv_all_once; ss; clarify. Qed.
+
+  Program Definition modsem2: ModSem.t :=
+    {|
+      ModSem.step := step2;
+      ModSem.at_external := at_external;
+      ModSem.initial_frame := initial_frame;
+      ModSem.final_frame := final_frame;
+      ModSem.after_external := after_external;
+      ModSem.globalenv := ge;
+      ModSem.skenv := skenv;
+    |}
+  .
+  Next Obligation. ii; ss; des. inv_all_once; ss; clarify. Qed.
+  Next Obligation. ii; ss; des. inv_all_once; ss; clarify. Qed.
+  Next Obligation. ii; ss; des. inv_all_once; ss; clarify. f_equal. determ_tac typify_c_dtm. Qed.
+  Next Obligation. ii; ss; des. inv_all_once; ss; clarify. Qed.
+  Next Obligation. ii; ss; des. inv_all_once; ss; clarify. Qed.
+  Next Obligation. ii; ss; des. inv_all_once; ss; clarify. Qed.
+
+  Let lift_receptive: forall
+        (RECEP: receptive (semantics1_with_ge p ge))
+    ,
+      receptive modsem1
+  .
+  Proof. i.
+    inv RECEP. econs; eauto; ii; ss. exploit sr_receptive; eauto.
+    eapply match_traces_preserved; try eassumption. ii; ss.
+  Qed.
+
+  Lemma modsem1_receptive
+    :
+      receptive modsem1
+  .
+  Proof. admit "this should hold". Qed.
+
+  Lemma modsem1_determinate
+    :
+      determinate modsem1
+  .
+  Proof. admit "this should hold". Qed.
+
+  Lemma modsem2_receptive
+    :
+      receptive modsem2
+  .
+  Proof. admit "this should hold". Qed.
+
+  Lemma modsem2_determinate
+    :
+      determinate modsem2
+  .
+  Proof. admit "this should hold". Qed.
+
+End MODSEM.
+
+
+
+
+
+Section MODULE.
+
+  Variable p: program.
+
+  Program Definition module1: Mod.t :=
+    {|
+      Mod.data := p;
+      Mod.get_sk := CtypesC.of_program signature_of_function;
+      Mod.get_modsem := modsem1;
+    |}
+  .
+  Next Obligation.
+    rewrite CtypesC.of_program_defs. ss.
+  Qed.
+
+  Program Definition module2: Mod.t :=
+    {|
+      Mod.data := p;
+      Mod.get_sk := CtypesC.of_program signature_of_function;
+      Mod.get_modsem := modsem2;
+    |}
+  .
+  Next Obligation.
+    rewrite CtypesC.of_program_defs. ss.
+  Qed.
+
+End MODULE.
+
