cfrontend/CtypesC.v
@@ -1,9 +1,11 @@
 Require Import Axioms CoqlibC Maps Errors.
 Require Import AST Linking.
 Require Archi.
-
-Require Export Ctypes Csem Csyntax ASTC.
+(** newly added **)
+Require Export Ctypes.
+(* Csem Csyntax ASTC. *)
 Require Import Errors.
+Require Import Values.
 Require Import sflib.
 Require Import Skeleton ASTC.
 
@@ -55,11 +57,6 @@ Section CSPECIFIC.
     u in *. des_ifs.
   Qed.
 
-  Definition signature_of_function (f: function) :=
-    {| sig_args := typlist_of_typelist (type_of_params (fn_params f));
-       sig_res  := opttyp_of_type (fn_return f);
-       sig_cc   := fn_callconv f |}.
-
   Definition of_program {F} (get_sg: F -> signature) (prog: Ctypes.program F): Sk.t :=
     mkprogram (skdefs_of_gdefs get_sg (map (update_snd (@globdef_of_globdef F type)) prog.(prog_defs))) prog.(prog_public) prog.(prog_main)
   .
@@ -82,3 +79,4 @@ Section CSPECIFIC.
   Qed.
 
 End CSPECIFIC.
+
